A model of readable input buffers (does not extract)

src/3d/prelude/EverParse3d.Readable.fst
@@ -38,6 +38,8 @@ let loc_perm_gsub #t #b p offset length = ()
 
 let valid_perm_gsub h #t #b p offset length = ()
 
+let loc_perm_from_to_disjoint #t #b p from1 to1 from2 to2 = ()
+
 let readable h #t #b p from to =
   valid_perm h p /\
   B.as_seq h (B.gsub p from (to `U32.sub` from)) `Seq.equal` Seq.create (U32.v to - U32.v from) (G.hide true)
@@ -50,6 +52,37 @@ let readable_split h #t #b p from mid to =
   Seq.lemma_split (B.as_seq h (B.gsub b from (to `U32.sub` from))) (U32.v mid - U32.v from);
   Seq.lemma_split (B.as_seq h (B.gsub p from (to `U32.sub` from))) (U32.v mid - U32.v from)
 
-let loc_perm_from_to_disjoint #t #b p from1 to1 from2 to2 = ()
-
 let readable_frame h #t #b p from to l h' = ()
+
+let unreadable h #t #b p from to =
+  valid_perm h p ==>
+  B.as_seq h (B.gsub p from (to `U32.sub` from)) `Seq.equal` Seq.create (U32.v to - U32.v from) (G.hide false)
+
+let unreadable_prop h #t #b p from to = ()
+
+let readable_not_unreadable h #t #b p from to =
+  let f () : Lemma
+    (requires (readable h p from to /\ unreadable h p from to))
+    (ensures False)
+  = assert (valid_perm h p);
+    let s = B.as_seq h (B.gsub p from (to `U32.sub` from)) in
+    assert (s == Seq.create (U32.v to - U32.v from) (G.hide true));
+    assert (Seq.index s 0 == G.hide true);
+    assert (s == Seq.create (U32.v to - U32.v from) (G.hide false));
+    assert (Seq.index s 0 == G.hide false);
+    assert False
+  in
+  Classical.move_requires f ()
+
+let unreadable_gsub h #t #b p offset length from to = ()
+
+let unreadable_split h #t #b p from mid to =
+  Seq.lemma_split (B.as_seq h (B.gsub b from (to `U32.sub` from))) (U32.v mid - U32.v from);
+  Seq.lemma_split (B.as_seq h (B.gsub p from (to `U32.sub` from))) (U32.v mid - U32.v from)
+
+let unreadable_empty h #t #b p i = ()
+
+let unreadable_frame h #t #b p from to l h' = ()
+
+let scrub #t #b p from to =
+  B.fill (B.sub p from (to `U32.sub` from)) (G.hide false) (to `U32.sub` from)
