src/3d/prelude/EverParse3d.InputBuffer.fst
@@ -1,0 +1,41 @@
+module EverParse3d.InputBuffer
+
+module B = LowStar.Buffer
+module HS = FStar.HyperStack
+module HST = FStar.HyperStack.ST
+module U32 = FStar.UInt32
+module LPL = LowParse.Low.Base
+module R = EverParse3d.Readable
+module G = FStar.Ghost
+
+open LowParse.Low.Base
+
+noeq
+type input_buffer_t = {
+  slice: LPL.slice triv triv;
+  perm: R.perm slice.LPL.base;
+}
+
+let slice_of x = x.slice
+
+let slice_length x = x.slice.LPL.len
+
+let perm_of x = x.perm
+
+let truncate_input_buffer x len = {
+  slice = { base = x.slice.LPL.base; len = len; };
+  perm = x.perm;
+}
+
+let scrub sl from to =
+  R.scrub sl.perm from to
+
+let read_with_perm #k #t #p r j sl pos =
+  let pos' = j sl.slice pos in
+  scrub sl pos pos' ;
+  r sl.slice pos
+
+let puint8 = B.buffer LPL.byte
+
+let offset sl off =
+  B.moffset triv sl.slice.base off
