src/3d/prelude/EverParse3d.Readable.fsti
@@ -4,6 +4,7 @@ module B = LowStar.Buffer
 module HS = FStar.HyperStack
 module HST = FStar.HyperStack.ST
 module U32 = FStar.UInt32
+module LPL = LowParse.Low.Base
 
 inline_for_extraction noextract
 val perm (#t: Type) (b: B.buffer t) : Tot Type0
@@ -21,7 +22,8 @@ val valid_perm_prop (h: HS.mem) (#t: _) (#b: B.buffer t) (p: perm b)
   (requires (valid_perm h p))
   (ensures (
     B.live h b /\
-    B.loc_buffer b `B.loc_disjoint` loc_perm p
+    B.loc_buffer b `B.loc_disjoint` loc_perm p /\
+    loc_perm p `B.loc_in` h
   ))
   [SMTPat (valid_perm h p)]
 
@@ -40,6 +42,27 @@ val valid_perm_frame
   (ensures (
     valid_perm h' p
   ))
+
+let valid_perm_frame_pat
+  (h: HS.mem)
+  (#t: _) (#b: B.buffer t) (p: perm b)
+  (l: B.loc)
+  (h' : HS.mem)
+: Lemma
+  (requires (
+    valid_perm h p /\
+    B.modifies l h h' /\
+    B.loc_disjoint (loc_perm p) l /\
+    B.live h' b // because nothing prevents b from being deallocated
+  ))
+  (ensures (
+    valid_perm h' p
+  ))
+  [SMTPatOr [
+    [ SMTPat (B.modifies l h h'); SMTPat (valid_perm h p) ] ;
+    [ SMTPat (B.modifies l h h'); SMTPat (valid_perm h' p) ] ;
+  ]]
+= valid_perm_frame h p l h'
 
 val perm_gsub
   (#t: _) (#b: B.buffer t) (p: perm b)
@@ -72,8 +95,6 @@ val perm_offset
     p' == perm_gsub p offset (B.len b `U32.sub` offset)
   ))
 
-module LP = LowParse.Low.Base
-
 val perm_gsub_gsub
   (#t: _) (#b: B.buffer t) (p: perm b)
   (offset1: U32.t)
@@ -82,7 +103,7 @@ val perm_gsub_gsub
   (length2: U32.t { U32.v offset2 + U32.v length2 <= U32.v length1 })
 : Lemma
   ( 
-    perm_gsub (perm_gsub p offset1 length1) offset2 length2 == LP.coerce (perm (B.gsub (B.gsub b offset1 length1) offset2 length2)) (perm_gsub p (offset1 `U32.add` offset2) length2)
+    perm_gsub (perm_gsub p offset1 length1) offset2 length2 == LPL.coerce (perm (B.gsub (B.gsub b offset1 length1) offset2 length2)) (perm_gsub p (offset1 `U32.add` offset2) length2)
   )
   [SMTPat (perm_gsub (perm_gsub p offset1 length1) offset2 length2)]
 
@@ -91,7 +112,7 @@ val perm_gsub_zero_length
 : Lemma
   (
     B.gsub b 0ul (B.len b) == b /\
-    perm_gsub p 0ul (B.len b) == LP.coerce (perm (B.gsub b 0ul (B.len b))) p
+    perm_gsub p 0ul (B.len b) == LPL.coerce (perm (B.gsub b 0ul (B.len b))) p
   )
 
 val loc_perm_gsub
@@ -102,6 +123,24 @@ val loc_perm_gsub
   (loc_perm p `B.loc_includes` loc_perm (perm_gsub p offset length))
   [SMTPat (loc_perm (perm_gsub p offset length))]
 
+let loc_perm_gsub_includes
+  (#t: _) (#b: B.buffer t) (p: perm b)
+  (offset1: U32.t)
+  (length1: U32.t)
+  (offset2: U32.t)
+  (length2: U32.t)
+: Lemma
+  (requires (
+    U32.v offset1 <= U32.v offset2 /\
+    U32.v offset2 + U32.v length2 <= U32.v offset1 + U32.v length1 /\
+    U32.v offset1 + U32.v length1 <= B.length b
+  ))
+  (ensures (
+    loc_perm (perm_gsub p offset1 length1) `B.loc_includes` loc_perm (perm_gsub p offset2 length2)
+  ))
+//  [SMTPat [loc_perm (perm_gsub p offset1 length1) `B.loc_includes` loc_perm (perm_gsub p offset2 length2)]]
+= perm_gsub_gsub p offset1 length1 (offset2 `U32.sub` offset1) length2
+
 val valid_perm_gsub
   (h: HS.mem)
   (#t: _) (#b: B.buffer t) (p: perm b)
@@ -111,6 +150,36 @@ val valid_perm_gsub
   (requires (valid_perm h p))
   (ensures (valid_perm h (perm_gsub p offset length)))
   [SMTPat (valid_perm h (perm_gsub p offset length))]
+
+let loc_perm_from_to
+  (#t: _) (#b: B.buffer t) (p: perm b)
+  (from: U32.t)
+  (to: U32.t { U32.v from <= U32.v to /\ U32.v to <= B.length b })
+: GTot B.loc
+= loc_perm (perm_gsub p from (to `U32.sub` from))
+
+val loc_perm_from_to_disjoint
+  (#t: _) (#b: B.buffer t) (p: perm b)
+  (from1: U32.t)
+  (to1: U32.t { U32.v from1 <= U32.v to1 /\ U32.v to1 <= B.length b })
+  (from2: U32.t)
+  (to2: U32.t { U32.v from2 <= U32.v to2 /\ U32.v to2 <= B.length b })
+: Lemma
+  (requires (U32.v to1 <= U32.v from2 \/ U32.v to2 <= U32.v from1))
+  (ensures (loc_perm_from_to p from1 to1 `B.loc_disjoint` loc_perm_from_to p from2 to2))
+  [SMTPat (loc_perm_from_to p from1 to1 `B.loc_disjoint` loc_perm_from_to p from2 to2)]
+
+let loc_perm_from_to_includes
+  (#t: _) (#b: B.buffer t) (p: perm b)
+  (from1: U32.t)
+  (to1: U32.t { U32.v from1 <= U32.v to1 /\ U32.v to1 <= B.length b })
+  (from2: U32.t)
+  (to2: U32.t { U32.v from1 <= U32.v from2 /\ U32.v from2 <= U32.v to2 /\ U32.v to2 <= U32.v to1 })
+: Lemma
+  (requires True)
+  (ensures (loc_perm_from_to p from1 to1 `B.loc_includes` loc_perm_from_to p from2 to2))
+  [SMTPat (loc_perm_from_to p from1 to1 `B.loc_includes` loc_perm_from_to p from2 to2)]
+= loc_perm_gsub_includes p from1 (to1 `U32.sub` from1) from2 (to2 `U32.sub` from2)
 
 val readable
   (h: HS.mem)
@@ -150,24 +219,6 @@ val readable_split
 : Lemma
   (readable h p from to <==> (readable h p from mid /\ readable h p mid to))
 
-let loc_perm_from_to
-  (#t: _) (#b: B.buffer t) (p: perm b)
-  (from: U32.t)
-  (to: U32.t { U32.v from <= U32.v to /\ U32.v to <= B.length b })
-: GTot B.loc
-= loc_perm (perm_gsub p from (to `U32.sub` from))
-
-val loc_perm_from_to_disjoint
-  (#t: _) (#b: B.buffer t) (p: perm b)
-  (from1: U32.t)
-  (to1: U32.t { U32.v from1 <= U32.v to1 /\ U32.v to1 <= B.length b })
-  (from2: U32.t)
-  (to2: U32.t { U32.v from2 <= U32.v to2 /\ U32.v to2 <= B.length b })
-: Lemma
-  (requires (U32.v to1 <= U32.v from2 \/ U32.v to2 <= U32.v from1))
-  (ensures (loc_perm_from_to p from1 to1 `B.loc_disjoint` loc_perm_from_to p from2 to2))
-  [SMTPat (loc_perm_from_to p from1 to1 `B.loc_disjoint` loc_perm_from_to p from2 to2)]
-
 val readable_frame
   (h: HS.mem)
   (#t: _) (#b: B.buffer t) (p: perm b)
@@ -185,22 +236,100 @@ val readable_frame
   (ensures (
     readable h' p from to
   ))
+  [SMTPatOr [
+    [ SMTPat (B.modifies l h h'); SMTPat (readable h p from to) ] ;
+    [ SMTPat (B.modifies l h h'); SMTPat (readable h' p from to) ] ;
+  ]]
 
-inline_for_extraction noextract
-val read_with_perm
-  (#k: LP.parser_kind)
-  (#t: Type u#0)
-  (#p: LP.parser k t)
-  (r: LP.leaf_reader p)
-  (sl: LP.slice (B.trivial_preorder _) (B.trivial_preorder _))
-  (slp: perm sl.LP.base)
-  (pos: U32.t)
-: HST.Stack t
-  (requires (fun h ->
-    LP.valid p h sl pos /\
-    readable h slp pos (LP.get_valid_pos p h sl pos)
+val unreadable
+  (h: HS.mem)
+  (#t: _) (#b: B.buffer t) (p: perm b)
+  (from: U32.t)
+  (to: U32.t { U32.v from <= U32.v to /\ U32.v to <= B.length b })
+: GTot Type0
+
+val unreadable_prop
+  (h: HS.mem)
+  (#t: _) (#b: B.buffer t) (p: perm b)
+  (from: U32.t)
+  (to: U32.t { U32.v from <= U32.v to /\ U32.v to <= B.length b })
+: Lemma
+  (requires (~ (valid_perm h p)))
+  (ensures (unreadable h p from to))
+  [SMTPat (readable h p from to)]
+
+val readable_not_unreadable
+  (h: HS.mem)
+  (#t: _) (#b: B.buffer t) (p: perm b)
+  (from: U32.t)
+  (to: U32.t { U32.v from < (* important: not equal *) U32.v to /\ U32.v to <= B.length b })
+: Lemma
+  (~ (readable h p from to /\ unreadable h p from to))
+
+val unreadable_gsub
+  (h: HS.mem)
+  (#t: _) (#b: B.buffer t) (p: perm b)
+  (offset: U32.t)
+  (length: U32.t { U32.v offset + U32.v length <= B.length b })
+  (from: U32.t)
+  (to: U32.t { U32.v from <= U32.v to /\ U32.v to <= U32.v length })
+: Lemma
+  (requires (valid_perm h p))
+  (ensures (unreadable h (perm_gsub p offset length) from to <==> unreadable h p (offset `U32.add` from) (offset `U32.add` to)))
+  [SMTPat (unreadable h (perm_gsub p offset length) from to)]
+
+val unreadable_split
+  (h: HS.mem)
+  (#t: _) (#b: B.buffer t) (p: perm b)
+  (from: U32.t)
+  (mid: U32.t)
+  (to: U32.t { U32.v from <= U32.v mid /\ U32.v mid <= U32.v to /\ U32.v to <= B.length b })
+: Lemma
+  (unreadable h p from to <==> (unreadable h p from mid /\ unreadable h p mid to))
+
+val unreadable_empty
+  (h: HS.mem)
+  (#t: _) (#b: B.buffer t) (p: perm b)
+  (i: U32.t { U32.v i <= B.length b })
+: Lemma
+  (unreadable h p i i)
+
+val unreadable_frame
+  (h: HS.mem)
+  (#t: _) (#b: B.buffer t) (p: perm b)
+  (from: U32.t)
+  (to: U32.t { U32.v from <= U32.v to /\ U32.v to <= B.length b })
+  (l: B.loc)
+  (h' : HS.mem)
+: Lemma
+  (requires (
+    B.modifies l h h' /\
+    (valid_perm h' p ==> (
+      valid_perm h p /\
+      unreadable h p from to /\
+      B.loc_disjoint (loc_perm_from_to p from to) l /\
+      B.live h' b // because nothing prevents b from being deallocated
+  ))))
+  (ensures (
+    unreadable h' p from to
   ))
-  (ensures (fun h res h' ->
-    B.modifies (loc_perm_from_to slp pos (LP.get_valid_pos p h sl pos)) h h' /\
-    res == LP.contents p h sl pos
+  [SMTPatOr [
+    [ SMTPat (B.modifies l h h'); SMTPat (unreadable h p from to) ] ;
+    [ SMTPat (B.modifies l h h'); SMTPat (unreadable h' p from to) ] ;
+  ]]
+
+inline_for_extraction
+noextract
+val scrub
+  (#t: _) (#b: B.buffer t) (p: perm b)
+  (from: U32.t)
+  (to: U32.t { U32.v from <= U32.v to /\ U32.v to <= B.length b })
+: HST.Stack unit
+  (requires (fun h ->
+    valid_perm h p
+  ))
+  (ensures (fun h _ h' ->
+    B.modifies (loc_perm_from_to p from to) h h' /\
+    valid_perm h' p /\
+    unreadable h' p from to
   ))
